draft rename lemma

Core/Ty/Structure.lean
@@ -1,5 +1,6 @@
 import LeanSubst
 import Core.Ty.Definition
+import Core.Ty.Substitution
 
 open LeanSubst
 
@@ -10,11 +11,14 @@ def Ty.spine : Ty -> Option (String × List Ty)
   (x, sp ++ [a])
 | _ => none
 
+def Ty.apply (t : Ty) : List Ty -> Ty
+| [] => t
+| .cons a tl => (t • a).apply tl
+
 def Ty.arity : Ty -> Nat
 | arrow _ _ B => B.arity + 1
 | ∀[_] P => P.arity + 1
 | _ => 0
-
 
 inductive TyTeleElem
 | kind (k  : Kind)
@@ -39,3 +43,59 @@ def Ty.mk_from_tele : TyTele -> Ty -> Ty
 | .cons (.kind K) tys, t =>
   let r := t.mk_from_tele tys
   ∀[K] r
+@[simp]
+theorem Ty.Spine.apply_subst {t : Ty} {sp : List Ty} : (t.apply sp)[σ] = (t[σ]).apply (sp.map (·[σ])) := by
+  induction sp generalizing t <;> simp [Ty.apply]
+  case cons hd tl ih => rw [ih]; simp
+
+@[simp]
+theorem Ty.Spine.app_eq :
+  (f • a).spine = some (x, sp)
+  <-> ∃ sp', sp = sp' ++ [a] ∧ f.spine = some (x, sp')
+:= by
+  apply Iff.intro <;> intro h
+  case _ =>
+    simp [Ty.spine] at h
+    rw [Option.bind_eq_some_iff] at h
+    rcases h with ⟨q, e1, e2⟩
+    rcases q with ⟨y, sp'⟩; simp at e2
+    rcases e2 with ⟨e2, e3⟩; subst e2 e3
+    rw [e1]; exists sp'
+  case _ =>
+    rcases h with ⟨sp', e1, e2⟩; subst e1
+    simp [Ty.spine]
+    rw [Option.bind_eq_some_iff]; apply Exists.intro (x, sp')
+    apply And.intro e2; simp
+
+theorem Ty.Spine.apply_type {t : Ty} : t.apply sp • a = t.apply (sp ++ [a]) := by
+  induction sp generalizing t <;> simp [Ty.apply]
+  case cons hd tl ih => rw [ih]
+
+theorem Ty.Spine.apply_eq
+  : t.spine = some (x, sp) -> t = (gt#x).apply sp
+:= by
+  intro h
+  fun_induction Ty.spine generalizing x sp <;> simp at *
+  case _ y =>
+    rcases h with ⟨e1, e2⟩; subst e1 e2
+    simp [Ty.apply]
+  case _ ih =>
+    rw [Option.bind_eq_some_iff] at h
+    rcases h with ⟨q, e1, e2⟩
+    rcases q with ⟨y, sp'⟩; simp at e2
+    rcases e2 with ⟨e2, e3⟩; subst e2 e3
+    rw [ih e1, apply_type]
+
+theorem Ty.Spine.apply_compose {t : Ty}
+  : t.spine = some (x, sp1) -> (t.apply sp2).spine = some (x, sp1 ++ sp2)
+:= by
+  intro h; induction sp2 generalizing t x sp1
+  simp [Ty.apply]; exact h
+  case _ a tl ih =>
+  have lem : (t • a).spine = some (x, sp1 ++ [a]) := by simp; exact h
+  replace ih := ih lem; simp at ih; exact ih
+
+@[simp]
+theorem Ty.Spine.apply_eta : ((gt#x).apply sp).spine = some (x, sp) := by
+  have lem := @apply_compose x [] sp gt#x (by simp [Ty.spine])
+  simp at lem; exact lem
